fairness/lawyer/obligations/obligations_fin_branch.v
@@ -38,14 +38,14 @@ Section FiniteBranching.
   Qed.
 
   Lemma exchanges_cp_next_states δ d':
-    list_approx (fun δ' => exists τ π d n, exchanges_cp δ τ δ' π d d' n). 
+    list_approx (fun δ' => exists π d n, exchanges_cp δ δ' π d d' n). 
   Proof using.
     set (new_cps :=
            '(π, d) ← elements $ ps_cps δ;
            n ← seq 0 (ps_exc_bound δ + 1);
            mret (ps_cps δ ∖ {[+ (π, d) +]} ⊎ n *: {[+ (π, d') +]})).
     exists (map (flip (update_cps) δ) new_cps). 
-    intros ? (?&?&?&?& STEP).
+    intros ? (?&?&?& STEP).
     inversion STEP; subst; simpl in *. simpl.
     apply elem_of_list_In. apply in_map_iff. eexists. simpl. split; [reflexivity|].
     subst new_cps. apply elem_of_list_In.
@@ -138,10 +138,10 @@ Section FiniteBranching.
   Qed.
 
   Lemma increases_eb_next_states δ:
-    list_approx (fun δ' => exists τ, increases_eb δ τ δ').
+    list_approx (fun δ' => increases_eb δ δ').
   Proof using.
     exists [update_eb (ps_exc_bound δ + 1) δ]. 
-    intros ? (? & STEP). apply elem_of_list_singleton. 
+    intros ? STEP. apply elem_of_list_singleton. 
     by inversion STEP. 
   Qed.
 
@@ -177,8 +177,8 @@ Section FiniteBranching.
   Section FinParams.
     Context (FINdeg: Finite Degree) (FINlvl: Finite Level).
 
-    Lemma loc_step_approx δ:
-      list_approx (fun δ' => exists τ, loc_step δ τ δ'). 
+    Lemma loc_step_ex_approx δ:
+      list_approx (fun δ' => loc_step_ex δ δ'). 
     Proof using FINlvl FINdeg.
       exists (
           proj1_sig (burns_cp_next_states δ) ++
@@ -189,33 +189,32 @@ Section FiniteBranching.
             proj1_sig (expects_ep_next_states δ) ++
             proj1_sig (increases_eb_next_states δ)
         ).
-      intros ? (?& STEP).
-      rewrite !elem_of_app. 
-      destruct STEP as [T|[T|[T|[T|[T|[T|T]]]]]]. 
-      - destruct T as (?&?&T). left.
-        destruct (burns_cp_next_states δ); eauto. 
-      - destruct T as (?&?&?&?&T). do 1 right. left.
-        apply elem_of_list_In, in_flat_map. setoid_rewrite <- elem_of_list_In.      
-        eexists. split.
-        { eapply elem_of_enum. Unshelve. eauto. }
-        destruct exchanges_cp_next_states; eauto.
-        eapply e; eauto. 
-      - destruct T as (?&T). do 2 right. left.
+      intros ? STEP.
+      rewrite !elem_of_app.
+      inv_loc_step_ex STEP.      
+      (* destruct STEP as [T|[T|[T|[T|[T|[T|T]]]]]].  *)
+      - left. destruct (burns_cp_next_states δ); eauto. 
+      - do 2 right. left.
         apply elem_of_list_In, in_flat_map. setoid_rewrite <- elem_of_list_In.      
         eexists. split.
         { eapply elem_of_enum. Unshelve. eauto. }
         destruct creates_signal_next_states; eauto.
-      - destruct T as (?&T). do 3 right. left.
+      - do 3 right. left.
         destruct sets_signal_next_states; eauto.
-      - destruct T as (?&?&?&?&T). do 4 right. left.
+      - do 4 right. left.
         apply elem_of_list_In, in_flat_map. setoid_rewrite <- elem_of_list_In.      
         eexists. split.
         { eapply elem_of_enum. Unshelve. eauto. }
         destruct creates_ep_next_states; eauto.
         eapply e; eauto. 
-      - destruct T as (?&?&?&T). do 5 right. left.
+      - do 5 right. left.
         destruct expects_ep_next_states; eauto.
         eapply e; eauto.
+      - do 1 right. left.
+        apply elem_of_list_In, in_flat_map. setoid_rewrite <- elem_of_list_In.      
+        eexists. split.
+        { eapply elem_of_enum. Unshelve. eauto. }
+        destruct exchanges_cp_next_states; eauto.
       - repeat right.
         destruct increases_eb_next_states; eauto.
     Qed.
@@ -225,8 +224,8 @@ Section FiniteBranching.
     Proof using FINlvl FINdeg.
       clear H1 H0 H. 
       red.
-      exists (flat_map (fun i => list_approx_repeat (fun δ1 δ2 => exists τ, loc_step δ1 τ δ2)
-                           loc_step_approx i δ) (seq 0 (LIM_STEPS + 2))).
+      exists (flat_map (fun i => list_approx_repeat (fun δ1 δ2 => loc_step_ex δ1 δ2)
+                           loc_step_ex_approx i δ) (seq 0 (LIM_STEPS + 2))).
       intros δ' [τ STEP]. apply elem_of_list_In, in_flat_map.
       setoid_rewrite <- elem_of_list_In.
       red in STEP. destruct STEP as (n & LE & REL). exists (n + 1). split. 
@@ -235,8 +234,8 @@ Section FiniteBranching.
       destruct REL as (? & STEPS & STEP).
       rewrite Nat.add_1_r. apply rel_compose_nsteps_next.
       eexists. split.
-      2: { destruct STEP as (?&?&?). eexists.
-           red. left. eauto. }
+      2: { destruct STEP as (?&?&?).
+           left. eexists. left. eauto. }
       eapply nsteps_impl; eauto.
       red. intros ???????. subst. eauto.
     Qed.
